\documentclass[11pt]{article}

\usepackage{../analysis}

\begin{document}

\coverpage{9}

% hw problem 1 -----------------------------------------------------------------

\newpage
\section*{Problem 1}
    \problem{
        Let $f: \R ^2 \to \R$ be defined by
        \[
        f(x,y) =
        \begin{cases}
            \frac{xy(x^2 - y^2)}{x^2 + y^2} & (x,y) \neq (0,0) \\
            0                               & (x,y) = (0,0)
        \end{cases}
        \]
        {\bf (a)} Show that $\partial f / \partial x$, $\partial f / \partial y$ exist for all $(x,y) \in \R ^2$ \\\\
        {\bf (b)} Show that both $\frac{\partial ^2 f(0,0)}{\partial x \partial y}$ and $\frac{\partial ^2 f(0,0)}{\partial y \partial x}$ exist but $\frac{\partial ^2 f(0,0)}{\partial x \partial y} \neq \frac{\partial ^2 f(0,0)}{\partial y \partial x}$
    }
    \proof{ \\\\
        {\bf (a)} For $(x,y) \neq (0,0)$ we can just compute the partial derivatives.
        Consider
        $$\frac{\partial f}{\partial x}
        = \frac{[y(x^2 - y^2) + 2xyx](x^2 + y^2) - xy(x^2 - y^2)2x}{(x^2 + y^2)^2}
        = \frac{(3x^2y - y^3)(x^2 + y^2) + 2x^2y^3 - 2x^4y}{(x^2 + y^2)^2}
        $$
        $$ \frac{\partial f}{\partial y}
        = \frac{[x(x^2 - y^2) - 2yxy](x^2 + y^2) - xy(x^2 - y^2)2y}{(x^2 + y^2)^2}
        = \frac{(x^3 - 2xy^2)(x^2 + y^2) + 2xy^4 - 2x^3y^2}{(x^2 + y^2)^2}
        $$
        Then for each partial evaluated at 0, we take a limit.
        First consider $\frac{\partial f}{\partial x} (0,0)$:
        \begin{align*}
            \frac{\partial f}{\partial x} (0,0) &= \lim _{x \to 0} \frac{f(x,0) - f(0,0)}{x-0} \\
            &= \lim _{x \to 0} \frac{\frac{x*0(x^2 - 0^2)}{x^2 + 0^2}}{x} \\
            &= \lim _{x \to 0} \frac{0}{x^2} \frac{1}{x} = \lim _{x \to 0} \frac{0}{x^3} = \lim _{x \to 0} \frac{0}{3!} = \lim _{x \to 0} 0 = 0
        \end{align*}
        where we used L'Hopitals rule three times.
        Now consider $\frac{\partial f}{\partial y} (0,0)$
        \begin{align*}
            \frac{\partial f}{\partial y} (0,0) &= \lim _{y \to 0} \frac{f(0,y) - f(0,0)}{y-0} \\
            &= \lim _{y \to 0} \frac{\frac{0*y(0^2 - y^2)}{0^2 + y^2}}{y} \\
            &= \lim _{y \to 0} \frac{0}{y^2} \frac{1}{y} = \lim _{y \to 0} \frac{0}{y^3} = \lim _{y \to 0} \frac{0}{3!} = \lim _{y \to 0} 0 = 0
        \end{align*}
        {\bf (b)} Now we must compute the mixed partials and show their nonequality.
        $$ \frac{\partial ^2 f (0,0)}{\partial x \partial y}
        = \frac{\partial}{\partial x} \left( \frac{\partial f}{\partial y} \right) (0,0)
        = \lim _{x \to 0} \frac{ \frac{\partial f(x,0)}{\partial y} - \frac{\partial f (0,0)}{\partial y} }{x-0}
        = \lim _{x \to 0} \frac{ x^5 / x^4 }{x}
        = \lim _{x \to 0} \frac{x^5}{x^5}
        = \lim _{x \to 0} 1
        = 1
        $$
        $$ \frac{\partial ^2 f (0,0)}{\partial y \partial x}
        = \frac{\partial}{\partial y} \left( \frac{\partial f}{\partial x} \right) (0,0)
        = \lim _{y \to 0} \frac{ \frac{\partial f(0,y)}{\partial x} - \frac{\partial f (0,0)}{\partial x} }{y-0}
        = \lim _{y \to 0} \frac{ -y^5 / y^4 }{y}
        = \lim _{y \to 0} \frac{-y^5}{y^5}
        = \lim _{y \to 0} -1
        = -1
        $$
        \begin{flushright} $\square$ \end{flushright}
    }

% hw problem 2 -----------------------------------------------------------------

\newpage
\section*{Problem 2}
    \problem{
        For any $x = (x_1, \ldots , x_n) \in \R ^n$ and any multi-index $\alpha = (\alpha _1, \ldots , \alpha _n)$, prove that $|x^\alpha| \leq |x|^{|\alpha|}$ where $x^\alpha = x_1^{\alpha _1} \cdots x_n^{\alpha _n}$, $|x| = \sqrt{x_1^2 + \cdots + x_n^2}$, and $|\alpha| = \alpha _1 + \cdots + \alpha _n$
    }
    \proof{
        With the defined operations, we have (crucially) that $x_i \leq \sqrt{x_i^2} \leq \sqrt{x_1^2 + \cdots + x_i^2 + \cdots + x_n^2} = |x|$.
        This implies that, for any $x_i$, we have $|x _i ^{\alpha _i}| \leq | |x| ^{\alpha _i} | = |x| ^{\alpha _i}$.
        This allows us to deduce the following:
        $$
        |x ^\alpha |
        = | x_1 ^{\alpha _1} \cdots x_n ^{\alpha _n} |
        = |x_1 ^{\alpha _1}| \cdots |x_n ^{\alpha _n}|
        \leq |x| ^{\alpha _1} \cdots |x|^{\alpha _n}
        = |x| ^{\alpha _1 + \cdots + \alpha _n}
        = |x| ^{|\alpha|}
        $$
        which was the goal!
        \begin{flushright} $\square$ \end{flushright}
    }
















\end{document}
